coq_translation/examples-from-rust-book/error_handling/unpacking_options_via_question_mark.v
@@ -14,6 +14,7 @@ Module Person.
   Class AssociatedFunction (name : string) (T : Set) : Set := {
     associated_function : T;
   }.
+  Arguments associated_function name {T AssociatedFunction}.
 End Person.
 Definition Person : Set := Person.t.
 
@@ -28,23 +29,36 @@ Module Job.
   Class AssociatedFunction (name : string) (T : Set) : Set := {
     associated_function : T;
   }.
+  Arguments associated_function name {T AssociatedFunction}.
 End Job.
 Definition Job : Set := Job.t.
 
 Module Impl__crate_clone_Clone_for_Job.
   Definition Self := Job.
   
+  Definition clone (self : ref Self) : Job :=
+    let _ := tt in
+    deref self.
+  
+  Global Instance M_clone : Method "clone" _ := {|
+    method := clone;
+  |}.
+  Global Instance AF_clone : Job.AssociatedFunction "clone" _ := {|
+    Job.associated_function := clone;
+  |}.
+  Global Instance
+    AFT_clone
+    :
+    _crate.clone.Clone.AssociatedFunction
+    "clone"
+    _
+    :=
+    {|
+    _crate.clone.Clone.associated_function := clone;
+  |}.
+  
   Global Instance I : _crate.clone.Clone.Class Self := {|
-    Definition clone (self : ref Self) : Job :=
-      let _ := tt in
-      deref self.
-    
-    Global Instance AF_clone : Job.AssociatedFunction "clone" _ := {|
-      Job.associated_function := clone;
-    |}.
-    Global Instance M_clone : Method "clone" _ := {|
-      method := clone;
-    |}.
+    _crate.clone.Clone.clone := clone;
   |}.
 End Impl__crate_clone_Clone_for_Job.
 
@@ -52,7 +66,7 @@ Module Impl__crate_marker_Copy_for_Job.
   Definition Self := Job.
   
   Global Instance I : _crate.marker.Copy.Class Self :=
-      _crate.marker.Copy.Build_Class _.
+    _crate.marker.Copy.Build_Class _.
 End Impl__crate_marker_Copy_for_Job.
 
 Module PhoneNumber.
@@ -70,24 +84,37 @@ Module PhoneNumber.
   Class AssociatedFunction (name : string) (T : Set) : Set := {
     associated_function : T;
   }.
+  Arguments associated_function name {T AssociatedFunction}.
 End PhoneNumber.
 Definition PhoneNumber : Set := PhoneNumber.t.
 
 Module Impl__crate_clone_Clone_for_PhoneNumber.
   Definition Self := PhoneNumber.
   
+  Definition clone (self : ref Self) : PhoneNumber :=
+    let _ := tt in
+    let _ := tt in
+    deref self.
+  
+  Global Instance M_clone : Method "clone" _ := {|
+    method := clone;
+  |}.
+  Global Instance AF_clone : PhoneNumber.AssociatedFunction "clone" _ := {|
+    PhoneNumber.associated_function := clone;
+  |}.
+  Global Instance
+    AFT_clone
+    :
+    _crate.clone.Clone.AssociatedFunction
+    "clone"
+    _
+    :=
+    {|
+    _crate.clone.Clone.associated_function := clone;
+  |}.
+  
   Global Instance I : _crate.clone.Clone.Class Self := {|
-    Definition clone (self : ref Self) : PhoneNumber :=
-      let _ := tt in
-      let _ := tt in
-      deref self.
-    
-    Global Instance AF_clone : PhoneNumber.AssociatedFunction "clone" _ := {|
-      PhoneNumber.associated_function := clone;
-    |}.
-    Global Instance M_clone : Method "clone" _ := {|
-      method := clone;
-    |}.
+    _crate.clone.Clone.clone := clone;
   |}.
 End Impl__crate_clone_Clone_for_PhoneNumber.
 
@@ -95,7 +122,7 @@ Module Impl__crate_marker_Copy_for_PhoneNumber.
   Definition Self := PhoneNumber.
   
   Global Instance I : _crate.marker.Copy.Class Self :=
-      _crate.marker.Copy.Build_Class _.
+    _crate.marker.Copy.Build_Class _.
 End Impl__crate_marker_Copy_for_PhoneNumber.
 
 Module ImplPerson.
@@ -118,6 +145,9 @@ Module ImplPerson.
       | Continue {| Continue.0 := val; |} => val
       end.
   
+  Global Instance M_work_phone_area_code : Method "work_phone_area_code" _ := {|
+    method := work_phone_area_code;
+  |}.
   Global Instance
     AF_work_phone_area_code
     :
@@ -127,9 +157,6 @@ Module ImplPerson.
     :=
     {|
     Person.associated_function := work_phone_area_code;
-  |}.
-  Global Instance M_work_phone_area_code : Method "work_phone_area_code" _ := {|
-    method := work_phone_area_code;
   |}.
 End ImplPerson.
 
