coq_translation/examples-from-rust-book/error_handling/wrapping_errors.v
@@ -24,86 +24,104 @@ Definition DoubleError := DoubleError.t.
 Module Impl__crate_fmt_Debug_for_DoubleError.
   Definition Self := DoubleError.
   
+  Definition fmt
+      (self : ref Self)
+      (f : mut_ref _crate.fmt.Formatter)
+      : _crate.fmt.Result :=
+    match self with
+    | DoubleError.EmptyVec => _crate.fmt.ImplFormatter.write_str f "EmptyVec"
+    | DoubleError.Parse (__self_0) =>
+      _crate.fmt.ImplFormatter.debug_tuple_field1_finish f "Parse" __self_0
+    end.
+  
+  Global Instance M_fmt : Method "fmt" _ := {|
+    method := fmt;
+  |}.
+  Global Instance AF_fmt : DoubleError.AssociatedFunction "fmt" _ := {|
+    DoubleError.associated_function := fmt;
+  |}.
+  Global Instance AFT_fmt : _crate.fmt.Debug.AssociatedFunction "fmt" _ := {|
+    _crate.fmt.Debug.associated_function := fmt;
+  |}.
+  
   Global Instance I : _crate.fmt.Debug.Class Self := {|
-    Definition fmt
-        (self : ref Self)
-        (f : mut_ref _crate.fmt.Formatter)
-        : _crate.fmt.Result :=
-      match self with
-      | DoubleError.EmptyVec => _crate.fmt.ImplFormatter.write_str f "EmptyVec"
-      | DoubleError.Parse (__self_0) =>
-        _crate.fmt.ImplFormatter.debug_tuple_field1_finish f "Parse" __self_0
-      end.
-    
-    Global Instance AF_fmt : DoubleError.AssociatedFunction "fmt" _ := {|
-      DoubleError.associated_function := fmt;
-    |}.
-    Global Instance M_fmt : Method "fmt" _ := {|
-      method := fmt;
-    |}.
+    _crate.fmt.Debug.fmt := fmt;
   |}.
 End Impl__crate_fmt_Debug_for_DoubleError.
 
 Module Impl_fmt_Display_for_DoubleError.
   Definition Self := DoubleError.
   
+  Definition fmt (self : ref Self) (f : mut_ref fmt.Formatter) : fmt.Result :=
+    match deref self with
+    | DoubleError.EmptyVec =>
+      method
+        "write_fmt"
+        f
+        (_crate.fmt.ImplArguments.new_v1
+          [ "please use a vector with at least one element" ]
+          [  ])
+    | DoubleError.Parse () =>
+      method
+        "write_fmt"
+        f
+        (_crate.fmt.ImplArguments.new_v1
+          [ "the provided string could not be parsed as int" ]
+          [  ])
+    end.
+  
+  Global Instance M_fmt : Method "fmt" _ := {|
+    method := fmt;
+  |}.
+  Global Instance AF_fmt : DoubleError.AssociatedFunction "fmt" _ := {|
+    DoubleError.associated_function := fmt;
+  |}.
+  Global Instance AFT_fmt : fmt.Display.AssociatedFunction "fmt" _ := {|
+    fmt.Display.associated_function := fmt;
+  |}.
+  
   Global Instance I : fmt.Display.Class Self := {|
-    Definition fmt (self : ref Self) (f : mut_ref fmt.Formatter) : fmt.Result :=
-      match deref self with
-      | DoubleError.EmptyVec =>
-        method
-          "write_fmt"
-          f
-          (_crate.fmt.ImplArguments.new_v1
-            [ "please use a vector with at least one element" ]
-            [  ])
-      | DoubleError.Parse () =>
-        method
-          "write_fmt"
-          f
-          (_crate.fmt.ImplArguments.new_v1
-            [ "the provided string could not be parsed as int" ]
-            [  ])
-      end.
-    
-    Global Instance AF_fmt : DoubleError.AssociatedFunction "fmt" _ := {|
-      DoubleError.associated_function := fmt;
-    |}.
-    Global Instance M_fmt : Method "fmt" _ := {|
-      method := fmt;
-    |}.
+    fmt.Display.fmt := fmt;
   |}.
 End Impl_fmt_Display_for_DoubleError.
 
 Module Impl_error_Error_for_DoubleError.
   Definition Self := DoubleError.
   
+  Definition source (self : ref Self) : Option :=
+    match deref self with
+    | DoubleError.EmptyVec => None
+    | DoubleError.Parse (e) => Some e
+    end.
+  
+  Global Instance M_source : Method "source" _ := {|
+    method := source;
+  |}.
+  Global Instance AF_source : DoubleError.AssociatedFunction "source" _ := {|
+    DoubleError.associated_function := source;
+  |}.
+  Global Instance AFT_source : error.Error.AssociatedFunction "source" _ := {|
+    error.Error.associated_function := source;
+  |}.
+  
   Global Instance I : error.Error.Class Self := {|
-    Definition source (self : ref Self) : Option :=
-      match deref self with
-      | DoubleError.EmptyVec => None
-      | DoubleError.Parse (e) => Some e
-      end.
-    
-    Global Instance AF_source : DoubleError.AssociatedFunction "source" _ := {|
-      DoubleError.associated_function := source;
-    |}.
-    Global Instance M_source : Method "source" _ := {|
-      method := source;
-    |}.
   |}.
 End Impl_error_Error_for_DoubleError.
 
 Module Impl_From_for_DoubleError.
   Definition Self := DoubleError.
   
+  Definition from (err : ParseIntError) : DoubleError := DoubleError.Parse err.
+  
+  Global Instance AF_from : DoubleError.AssociatedFunction "from" _ := {|
+    DoubleError.associated_function := from;
+  |}.
+  Global Instance AFT_from : From.AssociatedFunction "from" _ := {|
+    From.associated_function := from;
+  |}.
+  
   Global Instance I : From.Class ParseIntError Self := {|
-    Definition from (err : ParseIntError) : DoubleError :=
-      DoubleError.Parse err.
-    
-    Global Instance AF_from : DoubleError.AssociatedFunction "from" _ := {|
-      DoubleError.associated_function := from;
-    |}.
+    From.from := from;
   |}.
 End Impl_From_for_DoubleError.
 
