coq_translation/examples-from-rust-book/functions/associated_functions_and_methods.v
@@ -18,6 +18,7 @@ Module Point.
   Class AssociatedFunction (name : string) (T : Set) : Set := {
     associated_function : T;
   }.
+  Arguments associated_function name {T AssociatedFunction}.
 End Point.
 Definition Point : Set := Point.t.
 
@@ -54,6 +55,7 @@ Module Rectangle.
   Class AssociatedFunction (name : string) (T : Set) : Set := {
     associated_function : T;
   }.
+  Arguments associated_function name {T AssociatedFunction}.
 End Rectangle.
 Definition Rectangle : Set := Rectangle.t.
 
@@ -63,11 +65,11 @@ Module ImplRectangle.
   Definition get_p1 (self : ref Self) : Point :=
     NamedField.get (name := "p1") self.
   
-  Global Instance AF_get_p1 : Rectangle.AssociatedFunction "get_p1" _ := {|
-    Rectangle.associated_function := get_p1;
-  |}.
   Global Instance M_get_p1 : Method "get_p1" _ := {|
     method := get_p1;
+  |}.
+  Global Instance AF_get_p1 : Rectangle.AssociatedFunction "get_p1" _ := {|
+    Rectangle.associated_function := get_p1;
   |}.
   
   Definition area (self : ref Self) : f64 :=
@@ -77,11 +79,11 @@ Module ImplRectangle.
       NamedField.get (name := "p2") self in
     method "abs" (mul (sub x1 x2) (sub y1 y2)).
   
-  Global Instance AF_area : Rectangle.AssociatedFunction "area" _ := {|
-    Rectangle.associated_function := area;
-  |}.
   Global Instance M_area : Method "area" _ := {|
     method := area;
+  |}.
+  Global Instance AF_area : Rectangle.AssociatedFunction "area" _ := {|
+    Rectangle.associated_function := area;
   |}.
   
   Definition perimeter (self : ref Self) : f64 :=
@@ -91,6 +93,9 @@ Module ImplRectangle.
       NamedField.get (name := "p2") self in
     mul 2 (* 2.0 *) (add (method "abs" (sub x1 x2)) (method "abs" (sub y1 y2))).
   
+  Global Instance M_perimeter : Method "perimeter" _ := {|
+    method := perimeter;
+  |}.
   Global Instance
     AF_perimeter
     :
@@ -100,9 +105,6 @@ Module ImplRectangle.
     :=
     {|
     Rectangle.associated_function := perimeter;
-  |}.
-  Global Instance M_perimeter : Method "perimeter" _ := {|
-    method := perimeter;
   |}.
   
   Definition translate (self : mut_ref Self) (x : f64) (y : f64) :=
@@ -128,6 +130,9 @@ Module ImplRectangle.
         y) ;;
     tt.
   
+  Global Instance M_translate : Method "translate" _ := {|
+    method := translate;
+  |}.
   Global Instance
     AF_translate
     :
@@ -137,9 +142,6 @@ Module ImplRectangle.
     :=
     {|
     Rectangle.associated_function := translate;
-  |}.
-  Global Instance M_translate : Method "translate" _ := {|
-    method := translate;
   |}.
 End ImplRectangle.
 
@@ -170,11 +172,11 @@ Module ImplPair.
     tt ;;
     tt.
   
-  Global Instance AF_destroy : Pair.AssociatedFunction "destroy" _ := {|
-    Pair.associated_function := destroy;
-  |}.
   Global Instance M_destroy : Method "destroy" _ := {|
     method := destroy;
+  |}.
+  Global Instance AF_destroy : Pair.AssociatedFunction "destroy" _ := {|
+    Pair.associated_function := destroy;
   |}.
 End ImplPair.
 
