coq_translation/examples-from-rust-book/scoping_rules/scoping_rules_ownership_and_rules_partial_moves.v
@@ -20,30 +20,36 @@ Module Person.
   Class AssociatedFunction (name : string) (T : Set) : Set := {
     associated_function : T;
   }.
+  Arguments associated_function name {T AssociatedFunction}.
 End Person.
 Definition Person : Set := Person.t.
 
 Module Impl__crate_fmt_Debug_for_Person.
   Definition Self := Person.
   
+  Definition fmt
+      (self : ref Self)
+      (f : mut_ref _crate.fmt.Formatter)
+      : _crate.fmt.Result :=
+    _crate.fmt.ImplFormatter.debug_struct_field2_finish
+      f
+      "Person"
+      "name"
+      (NamedField.get (name := "name") self)
+      "age"
+      (NamedField.get (name := "age") self).
+  
+  Global Instance M_fmt : Method "fmt" _ := {|
+    method := fmt;
+  |}.
+  Global Instance AF_fmt : Person.AssociatedFunction "fmt" _ := {|
+    Person.associated_function := fmt;
+  |}.
+  Global Instance AFT_fmt : _crate.fmt.Debug.AssociatedFunction "fmt" _ := {|
+    _crate.fmt.Debug.associated_function := fmt;
+  |}.
+  
   Global Instance I : _crate.fmt.Debug.Class Self := {|
-    Definition fmt
-        (self : ref Self)
-        (f : mut_ref _crate.fmt.Formatter)
-        : _crate.fmt.Result :=
-      _crate.fmt.ImplFormatter.debug_struct_field2_finish
-        f
-        "Person"
-        "name"
-        (NamedField.get (name := "name") self)
-        "age"
-        (NamedField.get (name := "age") self).
-    
-    Global Instance AF_fmt : Person.AssociatedFunction "fmt" _ := {|
-      Person.associated_function := fmt;
-    |}.
-    Global Instance M_fmt : Method "fmt" _ := {|
-      method := fmt;
-    |}.
+    _crate.fmt.Debug.fmt := fmt;
   |}.
 End Impl__crate_fmt_Debug_for_Person.
