coq_translation/examples-from-rust-book/generics/generics_new_type_idiom.v
@@ -27,11 +27,11 @@ Module ImplYears.
   Definition to_days (self : ref Self) : Days :=
     Days.Build (mul (IndexedField.get (index := 0) self) 365).
   
-  Global Instance AF_to_days : Years.AssociatedFunction "to_days" _ := {|
-    Years.associated_function := to_days;
-  |}.
   Global Instance M_to_days : Method "to_days" _ := {|
     method := to_days;
+  |}.
+  Global Instance AF_to_days : Years.AssociatedFunction "to_days" _ := {|
+    Years.associated_function := to_days;
   |}.
 End ImplYears.
 
@@ -41,11 +41,11 @@ Module ImplDays.
   Definition to_years (self : ref Self) : Years :=
     Years.Build (div (IndexedField.get (index := 0) self) 365).
   
-  Global Instance AF_to_years : Days.AssociatedFunction "to_years" _ := {|
-    Days.associated_function := to_years;
-  |}.
   Global Instance M_to_years : Method "to_years" _ := {|
     method := to_years;
+  |}.
+  Global Instance AF_to_years : Days.AssociatedFunction "to_years" _ := {|
+    Days.associated_function := to_years;
   |}.
 End ImplDays.
 
