coq_translation/examples-from-rust-book/scoping_rules/scoping_rules_lifetimes_methods.v
@@ -21,11 +21,11 @@ Module ImplOwner.
       (add (IndexedField.get (index := 0) self) 1) ;;
     tt.
   
-  Global Instance AF_add_one : Owner.AssociatedFunction "add_one" _ := {|
-    Owner.associated_function := add_one;
-  |}.
   Global Instance M_add_one : Method "add_one" _ := {|
     method := add_one;
+  |}.
+  Global Instance AF_add_one : Owner.AssociatedFunction "add_one" _ := {|
+    Owner.associated_function := add_one;
   |}.
   
   Definition print (self : ref Self) :=
@@ -39,11 +39,11 @@ Module ImplOwner.
     tt ;;
     tt.
   
-  Global Instance AF_print : Owner.AssociatedFunction "print" _ := {|
-    Owner.associated_function := print;
-  |}.
   Global Instance M_print : Method "print" _ := {|
     method := print;
+  |}.
+  Global Instance AF_print : Owner.AssociatedFunction "print" _ := {|
+    Owner.associated_function := print;
   |}.
 End ImplOwner.
 
